simplified

code01_simplified.dfy
@@ -2,7 +2,6 @@ datatype exp =
 | EInt(v: int)
 | EVar(x: string)
 | EAdd(e1: exp, e2: exp)
-| EMul(e1: exp, e2: exp)
 
 function eval(e: exp, env: string -> int): int
 {
@@ -10,7 +9,6 @@ function eval(e: exp, env: string -> int): int
     case EInt(v) => v
     case EVar(x) => env(x)
     case EAdd(e1, e2) => eval(e1, env) + eval(e2, env)
-    case EMul(e1, e2) => eval(e1, env) * eval(e2, env)
 }
 
 function optimize(e: exp): exp
@@ -19,17 +17,9 @@ function optimize(e: exp): exp
     case EInt(v) => e
     case EVar(x) => e
     case EAdd(e1, e2) => (match (optimize(e1), optimize(e2))
-        case (EInt(v1), EInt(v2)) => EInt(v1+v2)
         case (EInt(0), e2) => e2
         case (e1, EInt(0)) => e1
         case (e1, e2) => EAdd(e1, e2))
-    case EMul(e1, e2) => (match (optimize(e1), optimize(e2))
-        case (EInt(v1), EInt(v2)) => EInt(v1*v2)
-        case (EInt(0), e2) => EInt(0)
-        case (e1, EInt(0)) => EInt(0)
-        case (EInt(1), e2) => e2
-        case (e1, EInt(1)) => e1
-        case (e1, e2) => EMul(e1, e2))
 }
 
 lemma OptimizerPreservesSemantics(e: exp, env: string -> int)
@@ -42,16 +32,9 @@ predicate {:spec} optimal(e: exp)
     match e
     case EInt(_) => true
     case EVar(_) => true
-    case EAdd(EInt(_), EInt(_)) => false
     case EAdd(EInt(0), _) => false
     case EAdd(_, EInt(0)) => false
     case EAdd(e1, e2) => optimal(e1) && optimal(e2)
-    case EMul(EInt(_), EInt(_)) => false
-    case EMul(EInt(0), _) => false
-    case EMul(_, EInt(0)) => false
-    case EMul(EInt(1), _) => false
-    case EMul(_, EInt(1)) => false
-    case EMul(e1, e2) => optimal(e1) && optimal(e2)
 }
 
 lemma OptimizerIsOptimal(e: exp)
@@ -64,10 +47,6 @@ ensures optimal(optimize(e))
         case EVar(x) => {
         }
         case EAdd(e1, e2) => {
-            OptimizerIsOptimal(e1);
-            OptimizerIsOptimal(e2);
-        }
-        case EMul(e1, e2) => {
             OptimizerIsOptimal(e1);
             OptimizerIsOptimal(e2);
         }
